untyped lambda theory

theory/Lambda.thy
@@ -1,181 +1,480 @@
 theory Lambda
-imports Main
+imports Nominal
 begin
 
-fun pred :: "nat \<Rightarrow> nat" where
-  "pred 0 = 0"
-  | "pred (Suc k) = k"
+atom_decl name
 
 section {* lambda term with de Bruijn index *}
 
 subsection {* Definition *}
-datatype dlambda = lvar nat | labs dlambda | lapp dlambda dlambda
+
+nominal_datatype lambda =
+  Var "name"
+| App "lambda" "lambda"
+| Lam "\<guillemotleft>name\<guillemotright>lambda" ("lam [_]._" [100, 100] 100)
 
 notation
-  lapp (infixl "$" 60)
+  App (infixl "$" 120)
 
-subsection {* shift & subst *}
-fun shift' :: "(nat \<Rightarrow> nat) \<Rightarrow> nat \<Rightarrow> dlambda \<Rightarrow> dlambda" where
-  "shift' d c (lvar k) = (if k < c then lvar k else lvar (d k))"
-  | "shift' d c (labs t) = labs (shift' d (Suc c) t)"
-  | "shift' d c (lapp tx ty) = lapp (shift' d c tx) (shift' d c ty)"
+(* ascii code *)
 
-definition shift :: "(nat \<Rightarrow> nat) \<Rightarrow> dlambda \<Rightarrow> dlambda" where
-  "shift d M = shift' d 0 M"
+abbreviation nf where
+  "nf == name 102"
 
-fun subst :: "dlambda \<Rightarrow> nat \<Rightarrow> dlambda \<Rightarrow> dlambda" where
-  "subst (lvar k) j s = (if k = j then s else lvar k)"
-  | "subst (labs t) j s = labs (subst t (Suc j) (shift Suc s))"
-  | "subst (lapp t1 t2) j s = lapp (subst t1 j s) (subst t2 j s)"
+abbreviation np where
+  "np == name 112"
 
-definition subst_op ("_ [_ \<rightarrow> _]" [80] 70) where
-  "subst_op = subst"
+abbreviation nq where
+  "nq == name 113"
 
-fun subst0 :: "dlambda \<Rightarrow> dlambda \<Rightarrow> dlambda" where
-  "subst0 M N = shift pred (N [0 \<rightarrow> (shift Suc M)])"
-  
-value "subst0 (labs (lvar 10)) (lvar 0)"
+abbreviation nx where
+  "nx == name 120"
+
+abbreviation ny where
+  "ny == name 121"
+
+abbreviation nz where
+  "nz == name 122"
+
+subsubsection {* substitution *}  
+
+nominal_primrec subst :: "lambda \<Rightarrow> name \<Rightarrow> lambda \<Rightarrow> lambda" ("_[_::=_]") where
+  "(Var x)[y ::= s] = (if x = y then s else (Var x))"
+  | "(App M1 M2)[y ::= s] = App (M1[y ::= s]) (M2[y ::= s])"
+  | "x \<sharp> (y,s) \<Longrightarrow> (lam [x].M)[y ::= s] = lam [x].(M[y ::= s])"
+  apply (finite_guess)+
+  apply (rule TrueI)+
+  apply (simp add: abs_fresh)
+  apply (fresh_guess)+
+  done
+
+lemma forget:
+  assumes a: "x \<sharp> M"
+  shows "M [x ::= N] = M"
+using a
+apply (nominal_induct M avoiding: x N rule: lambda.strong_induct)
+apply (auto simp add: abs_fresh fresh_atm)
+done
+
+lemma fresh_fact:
+  fixes z :: "name"
+  assumes a: "z \<sharp> s" "z = y \<or> z \<sharp> t"
+  shows "z \<sharp> (t[y ::= s])"
+using a
+apply (nominal_induct t avoiding: z y s rule: lambda.strong_induct)
+apply (auto simp add: abs_fresh fresh_atm)
+done
+
+lemma subst:
+  assumes a: "x \<noteq> y" "x \<sharp> u"
+  shows "(t[x::=s][y::=u]) = (t[y::=u][x::=s[y::=u]])"
+using a
+apply (nominal_induct t avoiding: x y s u rule: lambda.strong_induct)
+apply (auto simp add: fresh_fact forget)
+done
+
+lemma subst_rename:
+  assumes a: "y \<sharp> t"
+  shows "(t[x::=s]) = (([(y,x)]\<bullet>t)[y::=s])"
+using a
+apply (nominal_induct t avoiding: x y s rule: lambda.strong_induct)
+apply (auto simp add: swap_simps fresh_atm abs_fresh)
+done
+
+subsection {* beta reduction *}
+
+inductive beta :: "lambda \<Rightarrow> lambda \<Rightarrow> bool" (infixl "\<rightarrow>\<beta>" 50) where
+  b_app1 [intro]: "t1 \<rightarrow>\<beta> t2 \<Longrightarrow> App t1 s \<rightarrow>\<beta> App t2 s"
+| b_app2 [intro]: "t1 \<rightarrow>\<beta> t2 \<Longrightarrow> App s t1 \<rightarrow>\<beta> App s t2"
+| b_abs [intro]: "t1 \<rightarrow>\<beta> t2 \<Longrightarrow> lam[x].t1 \<rightarrow>\<beta> lam[x].t2"
+| b_beta [intro]: "App (lam [x].t) s \<rightarrow>\<beta> (t[x::=s])"
+
+inductive long_beta :: "lambda \<Rightarrow> lambda \<Rightarrow> bool" (infixl "\<longrightarrow>\<beta>*" 50) where
+  bs_refl [intro]: "t \<longrightarrow>\<beta>* t"
+| bs_step [intro]: "t \<rightarrow>\<beta> s \<Longrightarrow> t \<longrightarrow>\<beta>* s"
+| bs_trans [trans]: "\<lbrakk> t1 \<longrightarrow>\<beta>* t2; t2 \<longrightarrow>\<beta>* t3 \<rbrakk> \<Longrightarrow> t1 \<longrightarrow>\<beta>* t3"
+
+inductive beta_eq :: "lambda \<Rightarrow> lambda \<Rightarrow> bool" (infixl "=\<beta>" 50) where
+  beq_bs [intro]: "t \<longrightarrow>\<beta>* s \<Longrightarrow> t =\<beta> s"
+| beq_sym [sym]: "t =\<beta> s \<Longrightarrow> s =\<beta> t"
+| beq_trans [trans]: "\<lbrakk> s =\<beta> t; t =\<beta> u \<rbrakk> \<Longrightarrow> s =\<beta> u"
+
+lemma bs_abs:
+  assumes "t1 \<longrightarrow>\<beta>* t2"
+  shows "\<And>x. lam [x]. t1 \<longrightarrow>\<beta>* lam [x]. t2"
+apply (rule long_beta.induct [OF assms], auto)
+apply (rule bs_trans, auto)
+done
+
+lemma bs_app1:
+  assumes "t1 \<longrightarrow>\<beta>* t2"
+  shows "\<And>s. App t1 s \<longrightarrow>\<beta>* App t2 s"
+apply (rule long_beta.induct [OF assms], auto)
+apply (rule bs_trans, auto)
+done
+
+lemma bs_app2:
+  assumes "t1 \<longrightarrow>\<beta>* t2"
+  shows "\<And>s. App s t1 \<longrightarrow>\<beta>* App s t2"
+apply (rule long_beta.induct [OF assms], auto)
+apply (rule bs_trans, auto)
+done
+
+lemma beq_refl [intro]: "t =\<beta> t"
+by (rule, rule bs_refl)
+
+lemma beq_app1:
+  assumes "t1 =\<beta> t2"
+  shows "\<And>s. App t1 s =\<beta> App t2 s"
+apply (rule beta_eq.induct [OF assms])
+apply (rule, rule bs_app1, simp)
+apply (rule beq_sym, simp)
+apply (rule beq_trans, simp, simp)
+done
+
+lemma beq_app2:
+  assumes "t1 =\<beta> t2"
+  shows "\<And>s. App s t1 =\<beta> App s t2"
+apply (rule beta_eq.induct [OF assms])
+apply (rule, rule bs_app2, simp)
+apply (rule beq_sym, simp)
+apply (rule beq_trans, simp, simp)
+done
 
 subsection {* free variables *}
 
-fun FV' :: "nat \<Rightarrow> dlambda \<Rightarrow> nat set" where
-  "FV' n (lvar x) = (if x \<ge> n then {x - n} else {})"
-  | "FV' n (lapp M N) = FV' n M \<union> FV' n N"
-  | "FV' n (labs M) = FV' (n+1) M"
+(*
+nominal_primrec FV :: "lambda \<Rightarrow> name set" where
+  "FV (Var x) = {x}"
+  | "FV (App M N) = FV M \<union> FV N"
+  | "FV (lam [x]. M) = FV M - {x}"
+  apply (finite_guess)+
+  apply simp+
+  defer
+  apply (fresh_guess)+
+  sorry
+*)
 
-definition FV :: "dlambda \<Rightarrow> nat set" where
-  "FV M = FV' 0 M"
-
-lemma "FV (lvar 0) = {0}" by (simp add: FV_def)
-lemma "FV (labs (lvar 0)) = {}" by (simp add: FV_def)
-lemma "FV (labs (labs (lapp (lvar 0) (lvar 10)))) = {8}" by (simp add: FV_def)
-
-subsubsection {* lemmas *}
-
-lemma subst'_nohit: "\<And>i N. 0 \<notin> FV' i M \<Longrightarrow> M [i \<rightarrow> N] = M"
-by (induction M, auto simp add: subst_op_def)
-
-lemma subst0_nohit: "\<And>N. 0 \<notin> FV M \<Longrightarrow> M [0 \<rightarrow> N] = M"
-by (simp add: subst'_nohit FV_def)
-
-lemma shift'_FV': "\<And>i j. i \<notin> FV' j (shift' (\<lambda>k. Suc (k + i)) j M)"
-by (induction M, auto)
-
-lemma shift_FV: "0 \<notin> FV (shift Suc M)"
-using shift'_FV' [of 0 0 M] by (simp add: shift_def FV_def)
-
-lemma shift_nosubst: "(shift Suc M) [0 \<rightarrow> N] = shift Suc M"
-by (rule subst0_nohit [OF shift_FV])
-
-lemma unshift'_shift'_id: "\<And>i. shift' pred (Suc i) (shift' Suc i M) = M"
-by (induction M, auto)
-
-lemma unshift'_shift'_i_Suci_id: "\<And>i. shift' pred i (shift' Suc i M) = M"
-by (induction M, auto)
-
-subsection {* closedness *} 
-
-definition closed :: "dlambda \<Rightarrow> bool" where
-  "closed M \<equiv> FV M = {}"
-
-lemma closed_subst_inv: "\<And>N. closed M \<Longrightarrow> M [0 \<rightarrow> N] = M"
-apply (rule subst0_nohit)
-by (simp add: closed_def)
-
-subsection {* reduction *}
-  
-inductive beta :: "dlambda \<Rightarrow> dlambda \<Rightarrow> bool" (infixl "=\<beta>" 50) where
-  b_beta: "beta (lapp (labs M) N) (subst0 N M)"
-| b_refl: "beta M M"
-| b_app1: "beta M M' \<Longrightarrow> beta (lapp M Z) (lapp M' Z)"
-| b_app2: "beta M M' \<Longrightarrow> beta (lapp Z M) (lapp Z M')"
-| b_abs: "beta M M' \<Longrightarrow> beta (labs M) (labs M')"
-| b_sym: "beta M N \<Longrightarrow> beta N M"
-| b_trans: "\<lbrakk> beta M N; beta N L \<rbrakk> \<Longrightarrow> beta M L"
-
-subsubsection {* Y combinator *}
+subsection {* fixedpoint *}
 
 definition Y where
-  "Y \<equiv> labs (lapp (labs (lapp (lvar 1) (lapp (lvar 0) (lvar 0)))) (labs (lapp (lvar 1) (lapp (lvar 0) (lvar 0)))))"
+  "Y \<equiv> lam [nf]. (lam [nx]. Var nf $ (Var nx $ Var nx)) $ (lam [nx]. Var nf $ (Var nx $ Var nx))"
 
-theorem fixedpoint_Y: "lapp Y M =\<beta> lapp M (lapp Y M)"
+theorem fixedpoint_Y:
+  assumes Mvar: "nx \<sharp> M"
+  shows "Y $ M =\<beta> M $ (Y $ M)"
 proof-
-  define X where "X = labs (lapp (lvar 1) (lapp (lvar 0) (lvar 0)))"
-  define M' where "M' = shift Suc M"
-  define W where "W = labs (lapp M' (lapp (lvar 0) (lvar 0)))"
-  have Y_is_lXX: "Y = labs (lapp X X)"
-    using Y_def X_def by simp
+  define X where "X = (lam [nx]. (Var nf $ (Var nx $ Var nx)))"
+  define W where "W = (lam [nx]. (M $ (Var nx $ Var nx)))"
+  have Y_is_lXX: "Y = (lam [nf]. (X $ X))"
+    apply (simp add: Y_def X_def)
+    done
+  have Mvar': "nx \<sharp> (nf,M)"
+    using Mvar
+    by (simp add: fresh_atm)
 
-  have H0: "beta (lapp Y M) (lapp (labs (lapp X X)) M)"
-    apply (subst Y_is_lXX)
-    by (rule b_refl)
-  have H1: "beta (lapp (labs (lapp X X)) M) (lapp W W)"
-    apply (rule, rule b_beta)
-    apply (simp add: X_def)
-    apply (simp add: unshift'_shift'_id shift_def subst_op_def)
-    apply (simp add: W_def M'_def shift_def)
-    by (rule b_refl)
-  have H2: "beta (lapp W W) (lapp (labs (lapp M' (lapp (lvar 0) (lvar 0)))) W)"
-    by (simp add: W_def, rule b_refl)
-  have H3: "beta (lapp (labs (lapp M' (lapp (lvar 0) (lvar 0)))) W) (lapp M (lapp W W))"
-    apply (rule, rule b_beta)
-    apply (simp add: M'_def)
-    using shift_nosubst [of M "shift Suc W"] apply (simp add: subst_op_def)
-    apply (simp add: unshift'_shift'_i_Suci_id shift_def)
-    by (rule b_refl)
-  have H4: "beta (lapp M (lapp Y M)) (lapp M (lapp W W))"
-    apply (rule b_app2)
-    by (rule, rule H0, rule H1)
+  have L0: "(lam [nx].Var nf $ (Var nx $ Var nx))[nf::=M] = W"
+    apply (simp add: W_def)
+    using Mvar' apply simp
+    done
+    
+  have H0: "Y $ M \<longrightarrow>\<beta>* (lam [nf]. (X $ X)) $ M"
+    by (subst Y_is_lXX, simp add: X_def, rule bs_refl)
+  also have H1: "(lam [nf]. (X $ X)) $ M \<longrightarrow>\<beta>* (lam [nx]. (M $ (Var nx $ Var nx))) $ W"
+    apply (simp add: X_def W_def)
+    apply (rule bs_trans, rule, rule b_beta)
+    apply (simp add: L0 W_def)
+    apply (rule bs_refl)
+    done
+  also have H2: "(lam [nx]. (M $ (Var nx $ Var nx))) $ W \<longrightarrow>\<beta>* M $ (W $ W)"
+    unfolding W_def
+    apply (rule bs_trans, rule, rule b_beta)
+    using forget [OF Mvar] apply simp
+    apply (rule bs_refl)
+    done
+  also have H3: "M $ (Y $ M) \<longrightarrow>\<beta>* M $ (W $ W)"
+    proof-
+      have H4: "Y $ M \<longrightarrow>\<beta>* W $ W"
+        apply (subst Y_is_lXX)
+        apply (rule bs_trans, rule H1, simp add: W_def, rule bs_refl)
+        done
+      show ?thesis
+        using bs_app2 [OF H4] by simp
+    qed
   show ?thesis
-    apply (rule, rule H0)
-    apply (rule, rule H1)
-    apply (rule, rule H2)
-    apply (rule, rule H3)
-    by (rule b_sym, rule H4)
-qed
+    apply (rule beq_trans, rule beq_bs)
+    apply (rule bs_trans [OF H0], rule bs_trans [OF H1], rule H2)
+    apply (rule beq_sym, rule, rule H3)
+    done
+qed        
 
 subsection {* definability *}
 
-primrec iter :: "(dlambda \<Rightarrow> dlambda) \<Rightarrow> nat \<Rightarrow> dlambda \<Rightarrow> dlambda" where
+primrec iter :: "(lambda \<Rightarrow> lambda) \<Rightarrow> nat \<Rightarrow> lambda \<Rightarrow> lambda" where
   "iter F 0 M = M"
   | "iter F (Suc i) M = F (iter F i M)"
 
+lemma iter_join: "iter F n (iter F m M) = iter F (n + m) M"
+by (induction n, auto)
+
 subsubsection {* Church number *}
 
-fun ChurchN :: "nat \<Rightarrow> dlambda" where
-  "ChurchN n = labs (labs (iter (\<lambda>k. lapp (lvar 1) k) n (lvar 0)))"
+fun ChurchN where
+  "ChurchN n = lam [nf]. lam [nx]. iter (\<lambda>k. Var nf $ k) n (Var nx)"
 
-lemma ChurchN_closed: "closed (ChurchN n)"
-apply (induction n)
-  apply (simp add: closed_def FV_def)
-by (simp add: closed_def FV_def)
+definition ChAdd where
+  "ChAdd = lam [nx]. lam [ny]. lam [np]. lam [nq]. Var nx $ Var np $ (Var ny $ Var np $ Var nq)"
+definition ChMult where
+  "ChMult = lam [nx]. lam [ny]. lam [nz]. Var nx $ (Var ny $ Var nz)"
+definition ChExp where
+  "ChExp = lam [nx]. lam [ny]. Var ny $ Var nx"
 
-definition ChAdd :: "dlambda" where
-  "ChAdd = labs (labs (labs (labs (lvar 3 $ lvar 1 $ (lvar 2 $ lvar 1 $ lvar 0)))))"
-definition ChMult :: "dlambda" where
-  "ChMult = labs (labs (labs (lvar 2 $ (lvar 1 $ lvar 0))))"
-definition ChExp :: "dlambda" where
-  "ChExp = labs (labs (lvar 0 $ lvar 1))"
+text {*
+  ChAdd n m
+  = (lam x. lam y. lam p. lam q. x p (y p q)) (lam f. lam x. iter (f -) n x) (lam f. lam x. iter (f -) m x)
+  = lam p. lam q. (lam f. lam x. iter (f -) n x) p ((lam f. lam x. iter (f -) m x) p q)
+  = lam p. lam q. (lam f. lam x. iter (f -) n x) p (iter (p -) m q))
+  = lam p. lam q. (iter (p -) n (iter (p -) m q))
+  = lam p. lam q. (iter (p -) (n + m) q)
+  = n + m
+*}
 
 lemma ChAdd_add: "ChAdd $ ChurchN n $ ChurchN m =\<beta> ChurchN (n + m)"
-proof (induction m)
-  case 0
-  have "ChAdd $ ChurchN n $ ChurchN 0 =\<beta> (labs (labs (labs (labs (lvar 3 $ lvar 1 $ (lvar 2 $ lvar 1 $ lvar 0)))))) $ ChurchN n $ ChurchN 0"
-    by (simp add: ChAdd_def, rule b_refl)
-  also have "((labs (labs (labs (labs (lvar 3 $ lvar 1 $ (lvar 2 $ lvar 1 $ lvar 0)))))) $ ChurchN n $ ChurchN 0) =\<beta> ((labs (labs (labs (ChurchN n $ lvar 1 $ (lvar 2 $ lvar 1 $ lvar 0))))) $ ChurchN 0)"
-    apply (rule b_app1)
-    apply (rule, rule b_beta)
-    
-next
-  case (Suc m)
-  then show ?case sorry
+proof-
+  have f1y: "ny \<sharp> (nx, ChurchN n)"
+    apply (induction n)
+      apply (simp add: abs_fresh fresh_atm)
+      apply (simp add: abs_fresh fresh_atm fresh_prod)
+    done
+  have f1p: "np \<sharp> (nx, ChurchN n)"
+    apply (induction n)
+      apply (simp add: abs_fresh fresh_atm)
+      apply (simp add: abs_fresh fresh_atm fresh_prod)
+    done
+  have f1q: "nq \<sharp> (nx, ChurchN n)"
+    apply (induction n)
+      apply (simp add: abs_fresh fresh_atm)
+      apply (simp add: abs_fresh fresh_atm fresh_prod)
+    done
+  have f2p: "np \<sharp> (ny, ChurchN m)"
+    apply (induction m)
+      apply (simp add: abs_fresh fresh_atm)
+      apply (simp add: abs_fresh fresh_atm fresh_prod)
+    done
+  have f2q: "nq \<sharp> (ny, ChurchN m)"
+    apply (induction m)
+      apply (simp add: abs_fresh fresh_atm)
+      apply (simp add: abs_fresh fresh_atm fresh_prod)
+    done
+  have f3f: "nf \<sharp> (ny, ChurchN m)"
+    apply (induction m)
+      apply (simp add: abs_fresh fresh_atm)
+      apply (simp add: abs_fresh fresh_atm fresh_prod)
+    done
+  have f3x: "nx \<sharp> (ny, ChurchN m)"
+    apply (induction m)
+      apply (simp add: abs_fresh fresh_atm)
+      apply (simp add: abs_fresh fresh_atm fresh_prod)
+    done
+  have f4x: "nx \<sharp> (nf, Var np)"
+    by (simp add: fresh_atm)
+
+  have "ChAdd $ (ChurchN n) $ (ChurchN m) \<longrightarrow>\<beta>* (lam [nx]. lam [ny]. lam [np]. lam [nq]. Var nx $ Var np $ (Var ny $ Var np $ Var nq)) $ (ChurchN n) $ (ChurchN m)"
+    by (simp add: ChAdd_def, rule bs_refl)
+  also have "... \<longrightarrow>\<beta>* (lam [ny]. lam [np]. lam [nq]. ChurchN n $ Var np $ (Var ny $ Var np $ Var nq)) $ (ChurchN m)"
+    apply (rule bs_app1, rule, rule, rule b_beta)
+    proof-
+      have h: "(lam [ny].lam [np].lam [nq].Var nx $ Var np $ (Var ny $ Var np $ Var nq))[nx::=ChurchN n] = lam [ny].lam [np].lam [nq].(ChurchN n $ Var np $ (Var ny $ Var np $ Var nq))"
+        apply (subst subst.simps(3) [OF f1y])
+        apply (subst subst.simps(3) [OF f1p])
+        apply (subst subst.simps(3) [OF f1q])
+        apply simp
+        done
+      show "(lam [ny].lam [np].lam [nq].Var nx $ Var np $ (Var ny $ Var np $ Var nq))[nx::=ChurchN n] \<longrightarrow>\<beta>* lam [ny].lam [np].lam [nq].ChurchN n $ Var np $ (Var ny $ Var np $ Var nq)"
+        by (subst h, rule bs_refl)
+    qed
+  also have "... \<longrightarrow>\<beta>* lam [np]. lam [nq]. ChurchN n $ Var np $ (ChurchN m $ Var np $ Var nq)"
+    apply (rule, rule, rule b_beta)
+    proof-
+      have h: "(lam [np].lam [nq].ChurchN n $ Var np $ (Var ny $ Var np $ Var nq))[ny::=ChurchN m] = lam [np].lam [nq].ChurchN n $ Var np $ (ChurchN m $ Var np $ Var nq)"
+        apply (subst subst.simps(3) [OF f2p])
+        apply (subst subst.simps(3) [OF f2q])
+        apply (subst lambda.inject(3), subst abs_fun_eq1)
+        apply (subst lambda.inject(3), subst abs_fun_eq1)
+        apply simp
+        using subst.simps(3) [OF f3f] subst.simps(3) [OF f3x]
+        by (smt ChurchN.simps f1y forget fresh_prodD(2))
+      show "(lam [np].lam [nq].ChurchN n $ Var np $ (Var ny $ Var np $ Var nq))[ny::=ChurchN m] \<longrightarrow>\<beta>* lam [np].lam [nq].ChurchN n $ Var np $ (ChurchN m $ Var np $ Var nq)"
+        by (subst h, rule bs_refl)
+    qed
+  also have "... = lam [np]. lam [nq]. ChurchN n $ Var np $ ((lam [nf]. lam [nx]. iter (\<lambda>k. Var nf $ k) m (Var nx)) $ Var np $ Var nq)" by simp
+  also have "... \<longrightarrow>\<beta>* lam [np]. lam [nq]. ChurchN n $ Var np $ (iter (\<lambda>k. Var np $ k) m (Var nq))"
+    apply (rule bs_abs, rule bs_abs, rule bs_app2)
+    apply (rule, rule, rule, rule b_beta)
+    apply (simp add: subst.simps(3) [OF f4x])
+    apply (rule bs_trans, rule, rule b_beta)
+    proof-
+      have h: "(iter (op $ (Var nf)) m (Var nx))[nf::=Var np][nx::=Var nq] = iter (op $ (Var np)) m (Var nq)"
+        by (induction m, auto)
+      show "(iter (op $ (Var nf)) m (Var nx))[nf::=Var np][nx::=Var nq] \<longrightarrow>\<beta>* iter (op $ (Var np)) m (Var nq)" 
+        by (subst h, rule bs_refl)
+    qed
+  also have "... = lam [np]. lam [nq]. (lam [nf]. lam [nx]. iter (\<lambda>k. Var nf $ k) n (Var nx)) $ Var np $ (iter (\<lambda>k. Var np $ k) m (Var nq))" by simp
+  also have "... \<longrightarrow>\<beta>* lam [np]. lam [nq]. (iter (\<lambda>k. Var np $ k) n (iter (\<lambda>k. Var np $ k) m (Var nq)))"
+    apply (rule bs_trans, rule bs_abs, rule bs_abs, rule bs_app1, rule, rule b_beta)
+    apply (simp add: subst.simps(3) [OF f4x])
+    apply (rule bs_abs, rule bs_abs)
+    apply (rule bs_trans, rule, rule b_beta)
+    proof-
+      have h: "(iter (op $ (Var nf)) n (Var nx))[nf::=Var np][nx::=iter (op $ (Var np)) m (Var nq)] \<longrightarrow>\<beta>* iter (op $ (Var np)) n (iter (op $ (Var np)) m (Var nq))"
+        apply (induction n, auto)
+        apply (rule bs_app2, simp)
+        done
+      show "(iter (op $ (Var nf)) n (Var nx))[nf::=Var np][nx::=iter (op $ (Var np)) m (Var nq)] \<longrightarrow>\<beta>* iter (op $ (Var np)) n (iter (op $ (Var np)) m (Var nq))"
+        by (simp add: h)
+    qed
+  also have "... = lam [np]. lam [nq]. (iter (\<lambda>k. Var np $ k) (n + m) (Var nq))" by (simp add: iter_join)
+  also have "... = lam [nf]. lam [nx]. (iter (\<lambda>k. Var nf $ k) (n + m) (Var nx))"
+    apply (subst lambda.inject(3), subst alpha)
+    apply (rule disjI2, rule, simp, rule)
+      apply (simp, subst swap_simps, simp, simp)
+    apply (subst lambda.inject(3), subst alpha)
+      apply (rule disjI2, rule, simp, rule)
+      apply (induction n, simp)
+        apply (induction m, simp add: swap_simps, simp add: swap_simps)
+        apply (induction m, simp add: swap_simps, simp add: swap_simps)
+    apply (induction n, simp)
+      apply (induction m, simp add: swap_simps fresh_atm, simp add: swap_simps fresh_atm)
+      apply (induction m, simp add: swap_simps fresh_atm, simp add: swap_simps fresh_atm)
+    apply (induction n, simp)
+      apply (induction m, simp add: swap_simps fresh_atm abs_fresh, simp add: swap_simps fresh_atm abs_fresh)
+      apply (induction m, simp add: swap_simps fresh_atm abs_fresh, simp add: swap_simps fresh_atm abs_fresh)
+    done
+  also have "... = ChurchN (n + m)" by simp
+  finally have lem: "(ChAdd $ ChurchN n $ ChurchN m) \<longrightarrow>\<beta>* ChurchN (n + m)" by simp
+
+  show ?thesis
+    by (rule, rule lem)
 qed
 
+subsubsection {* Boolean, conditional *}
 
+definition Btrue where
+  "Btrue = lam [nx]. lam [ny]. Var nx"
+definition Bfalse where
+  "Bfalse = lam [nx]. lam [ny]. Var ny"
 
+definition Bif where
+  "Bif b p q = b $ p $ q"
 
+lemma Bif_true:
+  assumes fp: "ny \<sharp> (nx, P)" "ny \<sharp> P"
+  shows "Bif Btrue P Q =\<beta> P"
+proof rule
+  have "Bif Btrue P Q = (lam [nx]. lam [ny]. Var nx) $ P $ Q"
+    by (simp add: Bif_def Btrue_def)
+  also have "... \<longrightarrow>\<beta>* (lam [ny]. P) $ Q"
+    apply (rule bs_app1, rule, rule, rule b_beta)
+    apply (subst subst.simps(3) [OF fp(1)], rule bs_abs, simp, rule bs_refl)
+    done
+  also have "... \<longrightarrow>\<beta>* P"
+    apply (rule, rule, rule b_beta)
+    apply (subst forget, rule fp, rule bs_refl)
+    done
+  finally show "Bif Btrue P Q \<longrightarrow>\<beta>* P" by simp
+qed
 
+lemma Bif_false:
+  assumes fp: "ny \<sharp> (nx, P)" "ny \<sharp> Q"
+  shows "Bif Bfalse P Q =\<beta> Q"
+proof rule
+  have "Bif Bfalse P Q = (lam [nx]. lam [ny]. Var ny) $ P $ Q"
+    by (simp add: Bif_def Bfalse_def)
+  also have "... \<longrightarrow>\<beta>* (lam [ny]. Var ny) $ Q"
+    apply (rule bs_app1, rule, rule, rule b_beta)
+    apply (subst subst.simps(3) [OF fp(1)], rule bs_abs, simp, rule bs_refl)
+    done
+  also have "... \<longrightarrow>\<beta>* Q"
+    apply (rule, rule, rule b_beta)
+    apply (simp, rule bs_refl)
+    done
+  finally show "Bif Bfalse P Q \<longrightarrow>\<beta>* Q" by simp
+qed
 
+subsubsection {* Pairing *}
+
+definition Ppair where
+  "Ppair M N = lam [nz]. Var nz $ M $ N"
+definition Pproj1 where
+  "Pproj1 M = M $ Btrue"
+definition Pproj2 where
+  "Pproj2 M = M $ Bfalse"
+
+lemma Ppair_proj1:
+  assumes "nz \<sharp> M" "nz \<sharp> N" "ny \<sharp> M"
+  shows "Pproj1 (Ppair M N) =\<beta> M"
+proof rule
+  have f1y: "ny \<sharp> (nx, M)"
+    apply (simp add: fresh_prod, rule)
+    apply (simp add: fresh_atm)
+    apply (rule assms)
+    done
+
+  have "Pproj1 (Ppair M N) = (lam [nz]. Var nz $ M $ N) $ Btrue"
+    by (simp add: Pproj1_def Ppair_def)
+  also have "... \<longrightarrow>\<beta>* (Btrue $ M $ N)"
+    apply (rule, rule, rule)
+    apply (simp, subst forget, rule assms, subst forget, rule assms)
+    apply (rule bs_refl)
+    done
+  also have "... = ((lam [nx]. lam [ny]. Var nx) $ M $ N)"
+    by (simp add: Btrue_def)
+  also have "... \<longrightarrow>\<beta>* (lam [ny]. M) $ N"
+    apply (rule bs_app1, rule, rule, rule)
+    apply (subst subst.simps, rule f1y, rule bs_abs, simp)
+    apply (rule bs_refl)
+    done
+  also have "... \<longrightarrow>\<beta>* M"
+    by (rule, rule, rule, subst forget, rule assms, rule bs_refl)
+  finally show "Pproj1 (Ppair M N) \<longrightarrow>\<beta>* M" by simp
+qed
+
+lemma Ppair_proj2:
+  assumes "nz \<sharp> M" "nz \<sharp> N" "ny \<sharp> M"
+  shows "Pproj2 (Ppair M N) =\<beta> N"
+proof rule
+  have f1y: "ny \<sharp> (nx, M)"
+    apply (simp add: fresh_prod, rule)
+    apply (simp add: fresh_atm)
+    apply (rule assms)
+    done
+
+  have "Pproj2 (Ppair M N) = (lam [nz]. Var nz $ M $ N) $ Bfalse"
+    by (simp add: Pproj2_def Ppair_def)
+  also have "... \<longrightarrow>\<beta>* (Bfalse $ M $ N)"
+    apply (rule, rule, rule)
+    apply (simp, subst forget, rule assms, subst forget, rule assms)
+    apply (rule bs_refl)
+    done
+  also have "... = ((lam [nx]. lam [ny]. Var ny) $ M $ N)"
+    by (simp add: Bfalse_def)
+  also have "... \<longrightarrow>\<beta>* (lam [ny]. Var ny) $ N"
+    apply (rule bs_app1, rule, rule, rule)
+    apply (subst subst.simps, rule f1y, rule bs_abs, simp)
+    apply (rule bs_refl)
+    done
+  also have "... \<longrightarrow>\<beta>* N"
+    by (rule, rule, rule, simp, rule bs_refl)
+  finally show "Pproj2 (Ppair M N) \<longrightarrow>\<beta>* N" by simp
+qed
+
+subsubsection {* numeric function *}
+
+definition L1defined where
+  "L1defined f F = (\<forall>n. (F $ ChurchN n) =\<beta> ChurchN (f n))"
+
+definition L1definable where
+  "L1definable f = (\<exists>F. L1defined f F)"
 
 
 
